Logic/Vorspiel/StrongRec.lean
@@ -1,0 +1,95 @@
+import Logic.Vorspiel.Computability
+
+attribute [-instance] WType.instEncodableWType Encodable.finPi Encodable.fintypeArrowOfEncodable
+
+open Encodable
+variable {α β γ σ : Type*} [Primcodable α] [Primcodable β] [Primcodable γ] [Primcodable σ]
+
+namespace Primrec
+
+lemma nat_rec'' {f : α → ℕ} {g : α → β} {h : α → ℕ → β → β}
+  (hf : Primrec f) (hg : Primrec g) (hh : Primrec₂ (fun a (p : ℕ × β) => h a p.1 p.2)) :
+  Primrec (fun a => @Nat.rec _ (g a) (h a) (f a)) := nat_rec' hf hg hh
+
+lemma list_bind {f : α → List β} {g : α → β → List σ} (hf : Primrec f) (hg : Primrec₂ g) :
+    Primrec (fun a => (f a).bind (g a)) := list_join.comp (list_map hf hg)
+
+lemma option_toList : Primrec (Option.toList : Option α → List α) := by
+  have : Primrec (fun a => [a] : α → List α) := list_cons.comp Primrec.id (const [])
+  exact (option_casesOn Primrec.id (const []) (this.comp₂ Primrec₂.right)).of_eq
+    (fun o => by rcases o <;> simp)
+
+lemma iterate {f : α → α} (hf : Primrec f) : Primrec₂ (f^[·] ·) := by
+  have : Primrec₂ (fun s a => s.rec a (fun _ => f) : ℕ → α → α) :=
+    to₂' (nat_rec' fst snd (hf.comp₂ (snd.comp₂ Primrec₂.right)))
+  exact this.of_eq (fun s a => by
+    induction' s with s ih <;> simp[*]; { exact Eq.symm (Function.iterate_succ_apply' f s a) })
+
+lemma list_take : Primrec₂ (List.take : ℕ → List α → List α) := by
+  have : Primrec₂ (fun s a => s.rec [] (fun n as => as ++ (a.get? n).toList) : ℕ → List α → List α) :=
+    to₂' (nat_rec' fst (const [])
+      (list_append.comp₂ (snd.comp₂ Primrec₂.right)
+        (option_toList.comp₂ $ list_get?.comp₂ (snd.comp₂ Primrec₂.left) (fst.comp₂ Primrec₂.right))))
+  exact this.of_eq (fun n as => by induction' n with n ih <;> simp[List.take_succ, *])
+
+private def iterateL (f : α → ℕ → β) (h : α → α) (a : α) (m k : ℕ) : List β :=
+  (List.range k).map (f (h^[m - k.pred] a))
+
+private def F (g : α × ℕ → List σ → Option σ) (h : α → α) (a : α) (m : ℕ) : ℕ → List σ := fun k =>
+  k.rec [] (fun k ih => (List.range k).bind (fun k' => (g (h^[m - k] a, k') (ih.take k')).toList) ++ (g (h^[m - k] a, k) ih).toList)
+
+private lemma F_primrec {g : α × ℕ → List σ → Option σ} {h : α → α} (hg : Primrec₂ g) (hh : Primrec h) :
+  Primrec₂ (fun a p => F g h a p.1 p.2 : α → ℕ × ℕ → List σ) :=
+  to₂' <| nat_rec'' (snd.comp snd) (const [])
+    (list_append.comp₂
+      (to₂' <| list_bind (list_range.comp $ fst.comp snd) (option_toList.comp₂ $ hg.comp₂
+        (Primrec₂.pair.comp₂
+          ((iterate hh).comp₂
+            (nat_sub.comp₂ (fst.comp₂ $ snd.comp₂ $ fst.comp₂ Primrec₂.left) (fst.comp₂ $ snd.comp₂ Primrec₂.left))
+            (fst.comp₂ $ fst.comp₂ Primrec₂.left))
+          Primrec₂.right) (list_take.comp₂ Primrec₂.right (snd.comp₂ $ snd.comp₂ Primrec₂.left))))
+      (option_toList.comp₂ $ hg.comp₂
+        (Primrec₂.pair.comp₂
+          ((iterate hh).comp₂
+            (nat_sub.comp₂ (fst.comp₂ $ snd.comp₂ Primrec₂.left) (fst.comp₂ Primrec₂.right))
+            (fst.comp₂ Primrec₂.left))
+          (fst.comp₂ Primrec₂.right))
+        (snd.comp₂ $ Primrec₂.right)))
+
+private lemma F_eq_iterateL {f : α → ℕ → σ} {g : α × ℕ → List σ → Option σ} {h : α → α}
+  (H : ∀ a k, g (a, k) ((List.range k).map (f (h a))) = some (f a k)) (a) {m k} (hm : k ≤ m + 1) :
+    F g h a m k = iterateL f h a m k := by
+  have F_succ : ∀ a m k,
+    F g h a m (k + 1) =
+    (List.range k).bind (fun k' => (g (h^[m - k] a, k') ((F g h a m k).take k')).toList) ++
+      (g (h^[m - k] a, k) $ F g h a m k).toList := by intro a m k; simp[F]
+  simp[iterateL]
+  induction' k with k ih generalizing a m
+  · simp[F]
+  · simp[F_succ, List.range_succ]
+    have ih' : F g h a m k = (List.range k).map (f $ h^[m - k.pred] a) := ih a (Nat.le_of_lt hm)    
+    have heq : k ≠ 0 → h (h^[m - k] a) = h^[m - k.pred] a := fun hk => by
+      rw[←Function.iterate_succ_apply' h, Nat.sub_pred (Nat.lt_succ.mp hm) hk]
+    apply congr_arg₂
+    · have : ∀ k' < k, g (h^[m - k] a, k') ((F g h a m k).take k') = some (f (h^[m - k] a) k')
+      { intro k' hk'
+        have H' : g (h^[m - k] a, k') ((List.range k').map (f (h^[m - k.pred] a))) = some (f (h^[m - k] a) k') :=
+          by simpa[heq (ne_zero_of_lt hk')] using H (h^[m - k] a) k'
+        rw[←H', ih', List.take_map_range, Nat.min_eq_right (le_of_lt hk')] }
+      exact List.bind_toList_some this
+    · simp; rw[ih']
+      by_cases hk : k = 0
+      · simpa[hk] using H (h^[m] a) 0
+      · simpa only [heq hk] using H (h^[m - k] a) k
+
+lemma nat_one_side_strong_rec {f : α → ℕ → σ} {g : α × ℕ → List σ → Option σ} {h : α → α}
+  (hg : Primrec₂ g) (hh : Primrec h)
+  (H : ∀ a k, g (a, k) ((List.range k).map (f (h a))) = some (f a k)) : Primrec₂ f := 
+  have : Primrec₂ (fun a m => (F g h a m (m + 1)).get? m) :=
+    list_get?.comp₂
+      ((F_primrec hg hh).comp₂ Primrec₂.left ((Primrec₂.pair.comp Primrec.id succ).comp₂ Primrec₂.right))
+      Primrec₂.right
+  Primrec₂.option_some_iff.1 <| this.of_eq <| fun a m => by
+    simp[F_eq_iterateL H a (le_refl $ m + 1), iterateL, List.get?_range (Nat.lt.base m)]
+
+end Primrec
