Logic/Vorspiel/W.lean
@@ -1,0 +1,451 @@
+import Logic.Vorspiel.Computability
+
+attribute [-instance] WType.instEncodableWType Encodable.finPi Encodable.fintypeArrowOfEncodable
+
+namespace WType
+
+open Encodable Primrec Primcodable UniformlyPrimcodable
+variable {α : Type*} {β : α → Type*}
+  [Primcodable α] [(a : α) → Fintype (β a)] [(a : α) → DecidableEq (β a)] [(a : α) → Primcodable (β a)] [PrimrecCard β]
+
+def elimOpt (γ : Type*) (fγ : (Σ a : α, β a → γ) → Option γ) : WType β → Option γ
+  | ⟨a, f⟩ => (toFinArrowOpt (fun b => elimOpt γ fγ (f b))).bind fun g => fγ ⟨a, g⟩
+
+def SubWType {α : Type*} (β : α → Type*)
+  [(a : α) → Fintype (β a)] [(a : α) → Primcodable (β a)] (n : ℕ) := { t : WType β // t.depth ≤ n }
+
+namespace SubWType
+
+def mk (a : α) (f : β a → SubWType β s) : SubWType β (s + 1) := ⟨⟨a, fun i => (f i).val⟩, by simp[depth]; intro b; exact (f b).property ⟩
+
+abbrev ofWType (w : WType β) (n) (h : w.depth ≤ n) : SubWType β n := ⟨w, h⟩
+
+@[simp] lemma depth_le (t : SubWType β n) : t.val.depth ≤ n := t.property
+
+def elim' (γ : Type*) (fγ : (Σ a : α, β a → γ) → γ) (s) : SubWType β s → γ := fun ⟨t, _⟩ => t.elim γ fγ 
+
+lemma elim_const {w₁ : SubWType β s₁} {w₂ : SubWType β s₂} (h : w₁.val = w₂.val) (γ) (fγ : (Σ a : α, β a → γ) → γ) : 
+    elim' γ fγ s₁ w₁ = elim' γ fγ s₂ w₂ := by
+  rcases w₁ with ⟨w, hw₁⟩
+  rcases w₂ with ⟨w, hw₂⟩
+  simp at h; rcases h with rfl
+  simp[elim']
+
+def equiv_zero : SubWType β 0 ≃ Empty where
+  toFun := fun ⟨x, h⟩ => False.elim (not_lt_of_ge h $ WType.depth_pos _)
+  invFun := by rintro ⟨⟩
+  left_inv := fun ⟨x, h⟩ => False.elim (not_lt_of_ge h $ WType.depth_pos _)
+  right_inv := by rintro ⟨⟩
+
+def equiv_succ : SubWType β (n + 1) ≃ (Σ a : α, β a → SubWType β n) where
+  toFun := fun ⟨t, h⟩ => by rcases t with ⟨a, f⟩; exact ⟨a, fun b => ⟨f b, by simp[WType.depth] at h; exact h b⟩⟩
+  invFun := fun ⟨a, f⟩ => ofWType (WType.mk a (fun b => (f b).val)) (n + 1) (by simp[depth])
+  left_inv := fun ⟨t, h⟩ => by rcases t with ⟨a, f⟩; simp
+  right_inv := fun ⟨a, f⟩ => by simp
+
+def primcodable_zero : Primcodable (SubWType β 0) := Primcodable.ofEquiv _ equiv_zero
+
+def primcodable_succ (n) (_ : Primcodable (SubWType β n)) : Primcodable (SubWType β (n + 1)) := Primcodable.ofEquiv _ equiv_succ
+
+instance _root_.Primcodable.SubWType (n : ℕ) : Primcodable (SubWType β n) := Nat.rec SubWType.primcodable_zero SubWType.primcodable_succ n
+
+@[simp] lemma decode_zero : (decode e : Option (SubWType β 0)) = none := by
+  rcases (decode e) with (_ | w)
+  · rfl
+  · exact Empty.elim (equiv_zero w)
+
+lemma decode_succ :
+  decode (α := SubWType β (s + 1)) e =
+  ((decode (α := α) e.unpair.1).bind
+    $ fun a => (decode (α := List (SubWType β s)) e.unpair.2).bind
+      $ fun l => (l.toVector (Fintype.card (β a))).map
+        $ fun v => ofWType ⟨a, fun b => (fintypeArrowEquivVector.symm v b).val⟩ _ (by simp[depth, Equiv.vectorEquivFin])) :=
+  calc
+    decode (α := SubWType β (s + 1)) e
+      = Option.map (fun x => ofWType ⟨x.fst, fun b => (x.snd b).val⟩ (s + 1) (by simp[depth]))
+        (decode e : Option ((a : α) × (β a → SubWType β s))) :=
+      by simp[Primcodable.SubWType, primcodable_succ, Primcodable.ofEquiv_toEncodable]
+         rw[Encodable.decode_ofEquiv equiv_succ, equiv_succ]; simp
+    _ = ((decode (Nat.unpair e).fst : Option α).bind
+          $ fun a => (decode (α := (β a → SubWType β s)) (Nat.unpair e).snd).map
+            $ fun x => ofWType (WType.mk a fun b => (x b).val) (s + 1) (by simp[depth])) :=
+      by simp[Encodable.decode_sigma_val, Option.map_bind', Function.comp]
+    _ = ((decode e.unpair.1 : Option α).bind
+        $ fun a => (decode (α := List (SubWType β s)) e.unpair.2).bind
+          $ fun l => (l.toVector (Fintype.card (β a))).map
+            $ fun v => ofWType ⟨a, fun b => (fintypeArrowEquivVector.symm v b).val⟩ _ (by simp[depth, Equiv.vectorEquivFin])) :=
+      by congr; funext a; rw[decode_fintypeArrow]; simp[Option.map_bind']; congr
+
+lemma encode_mk (a : α) (f : β a → WType β) (h) :
+    encode (ofWType ⟨a, f⟩ (s + 1) h) = (encode a).pair (encode $ fun b => encode (ofWType (f b) s (by simp[depth] at h; exact h b))) := by
+  simp[Primcodable.SubWType, primcodable_succ, Primcodable.ofEquiv_toEncodable]
+  rw[Encodable.encode_ofEquiv equiv_succ, equiv_succ]; simp[ofWType]
+  rw[Encodable.encode_sigma_val]
+  simp; exact encode_fintypeArrow' (β a) (SubWType β s) _
+
+section elimDecode
+
+variable {σ : Type*} {γ : Type*}
+variable (β)
+
+def elimDecode (f : α → List γ → γ) : ℕ → ℕ → Option γ :=
+ fun s e => (decode e : Option (SubWType β s)).map (elim' γ (fun ⟨a, v⟩ => f a (List.ofFn $ fintypeArrowEquivFinArrow v)) s)
+
+variable {β}
+
+abbrev decode' (s e : ℕ) : Option (SubWType β s) := decode e
+
+lemma elim'_eq_elimDecode [Inhabited γ] (f : (a : α) × (β a → γ) → γ) :
+    (decode e).map (elim' γ f s) = elimDecode β (fun a l => f ⟨a, fintypeArrowEquivFinArrow.symm (fun i => l.getI i)⟩) s e := by
+  simp[elimDecode]
+  rcases (decode e) with (_ | w) <;> simp
+  { congr; funext ⟨a, j⟩; simp; congr; funext b; simp }
+
+lemma elim'_eq_elimDecode' [Inhabited γ] (f : (a : α) × (β a → γ) → γ) :
+    (decode' s e).map (elim' γ f s) = elimDecode β (fun a l => f ⟨a, fintypeArrowEquivFinArrow.symm (fun i => l.getI i)⟩) s e :=
+  elim'_eq_elimDecode f
+
+variable (β)
+
+lemma elimDecode_eq_induction (f : α → List γ → γ) (s e) :
+    elimDecode β f s e =
+    Nat.casesOn s none
+      (fun s => (decode e.unpair.1 : Option α).bind
+        $ fun a => (((Denumerable.ofNat (List ℕ) e.unpair.2).mapM' (elimDecode β f s)).bind
+          $ fun l => if l.length = Fintype.card (β a) then some l else none).map
+            $ fun v => f a v) := by
+  rcases s with (_ | s)
+  · simp[elimDecode]
+  · simp[elimDecode, SubWType.decode_succ, Option.map_bind', decode_list, Function.comp, List.mapM'_option_map]; congr
+    funext a
+    rcases hw : List.mapM' (decode : ℕ → Option (SubWType β s)) (Denumerable.ofNat (List ℕ) e.unpair.2) with (_ | w) <;> simp
+    { simp[List.toVector]
+      by_cases hlw : w.length = Fintype.card (β a) <;> simp[hlw, elim, elim']
+      { simp[Vector.get_mk_eq_get, List.ofFn_get_eq_map]; congr
+        rw[Encodable.fintypeArrowEquivFinArrow_fintypeEquivFin (fun i =>
+          WType.elim γ (fun x => f x.fst (List.ofFn (fintypeArrowEquivFinArrow x.snd))) (w.get (i.cast hlw.symm)).val)];
+        rw[List.ofFn_get_eq_map (fun z => WType.elim γ (fun x => f x.fst (List.ofFn (fintypeArrowEquivFinArrow x.snd))) z.val) w];rfl } }
+
+@[reducible]
+private def elimDecodeG (f : σ → α → List γ → γ) : σ → ℕ × ℕ → List (Option γ) → Option γ := fun x (s, e) ih =>
+  Nat.casesOn s none
+    (fun s => (decode e.unpair.1 : Option α).bind
+      $ fun a => (((Denumerable.ofNat (List ℕ) e.unpair.2).mapM' (fun c => ih.getI (s.pair c))).bind
+        $ fun l => if l.length = Fintype.card (β a) then some l else none).map
+          $ fun v => f x a v)
+
+private lemma elimDecodeG_eq_elimDecode (f : σ → α → List γ → γ) (x s e) :
+    elimDecodeG β f x (s, e) ((List.range (s.pair e)).map (fun i => elimDecode β (f x) i.unpair.1 i.unpair.2)) = elimDecode β (f x) s e := by
+  simp[elimDecode_eq_induction β (f x) s e, elimDecodeG]
+  rcases s with (_ | s) <;> simp; congr
+  funext a
+  have : 
+    mapM' (fun c => ((List.range ((s + 1).pair e)).map $ fun i => elimDecode β (f x) i.unpair.fst i.unpair.snd).getI (s.pair c))
+      (Denumerable.ofNat (List ℕ) e.unpair.2) =
+    mapM' (elimDecode β (f x) s) (Denumerable.ofNat (List ℕ) e.unpair.2) :=
+  List.mapM'_eq_mapM'_of_eq _ (by
+  { intro c hc
+    have : s.pair c < (s + 1).pair e := by
+      have : c < e.unpair.2 := Denumerable.lt_of_mem_list _ _ hc
+      exact lt_of_lt_of_le (Nat.pair_lt_pair_right s this) (Nat.pair_le_pair_of_le (Nat.le_succ s) (Nat.unpair_right_le e))
+    simp[List.getI_map_range _ this] })
+  rw[this]
+
+variable [Primcodable σ] [Primcodable γ]
+
+private lemma elimDecodeG_primrec {f : σ → α × List γ → γ} (hf : Primrec₂ f) :
+    Primrec₂ (fun p ih => elimDecodeG β (fun x a ih => f x (a, ih)) p.1 p.2 ih : σ × (ℕ × ℕ) → List (Option γ) → Option γ) :=
+  by apply Primrec.nat_casesOn (fst.comp $ snd.comp fst) (const none)
+      (by apply option_bind (Primrec.decode.comp $ fst.comp $ Primrec.unpair.comp $ snd.comp $ snd.comp $ fst.comp fst)
+            (by apply option_map
+                  (option_bind
+                    (by apply option_list_mapM'
+                          (by apply (Primrec.ofNat _).comp $ snd.comp $ Primrec.unpair.comp $ snd.comp $ snd.comp $ fst.comp $ fst.comp $ fst)
+                          (Primrec.list_getI.comp (snd.comp $ fst.comp $ fst.comp fst)
+                                (Primrec₂.natPair.comp (snd.comp $ fst.comp fst) snd)).to₂)
+                    (Primrec.ite
+                          (Primrec.eq.comp (list_length.comp snd) (PrimrecCard.card_prim.comp $ snd.comp fst))
+                          (option_some.comp snd)
+                          (const none)).to₂)
+                  (hf.comp (fst.comp $ fst.comp $ fst.comp $ fst.comp fst) (Primrec.pair (snd.comp fst) snd)).to₂))
+
+lemma primrec_elimDecode_param {f : σ → α × List γ → γ} (hf : Primrec₂ f) :
+    Primrec₂ (fun x p => elimDecode β (fun a ih => f x (a, ih)) p.1 p.2 : σ → ℕ × ℕ → Option γ) := by
+  have : Primrec₂ (fun p ih => some $ elimDecodeG β (fun x a ih => f x (a, ih)) p.1 p.2 ih : σ × (ℕ × ℕ) → List (Option γ) → Option (Option γ)) :=
+    option_some.comp (elimDecodeG_primrec β hf)
+  exact nat_strong_rec'2 _ this (by simp[elimDecodeG_eq_elimDecode β])
+
+lemma primrec_elimDecode {f : α → List γ → γ} (hf : Primrec₂ f) :
+    Primrec₂ (fun s e => elimDecode β f s e : ℕ → ℕ → Option γ) :=
+  have : Primrec₂ (fun _ p => f p.1 p.2 : Unit → α × List γ → γ) := hf.comp (fst.comp snd) (snd.comp snd)
+  (primrec_elimDecode_param β this).comp₂ (const ()).to₂ (fst.pair snd)
+
+lemma primrec_elimDecode_param_comp {f : σ → α × List γ → γ} {g : σ → ℕ} {h : σ → ℕ} (hf : Primrec₂ f) (hg : Primrec g) (hh : Primrec h) :
+    Primrec (fun x => elimDecode β (fun a l => f x (a, l)) (g x) (h x) : σ → Option γ) :=
+  (primrec_elimDecode_param β hf).comp Primrec.id (hg.pair hh)
+
+end elimDecode
+
+lemma encode_eq_elim' : ∀ w : SubWType β s, encode w = elim' ℕ encode s w := by
+  { induction' s with s ih
+    · simp; intro ⟨w, h⟩; simpa using lt_of_lt_of_le (depth_pos w) h
+    · rintro ⟨⟨a, f⟩, hw⟩; simp[elim', elim, Primcodable.SubWType, primcodable_succ, Primcodable.ofEquiv_toEncodable]
+      rw[Encodable.encode_ofEquiv equiv_succ]
+      simp[equiv_succ, Encodable.encode_sigma_val]
+      suffices :
+        encode (⟨a, fun b => ofWType (f b) s (by simp[depth, Nat.succ_eq_add_one] at hw; exact hw b)⟩ : (a : α) × (β a → SubWType β s)) =
+        encode (⟨a, fun b => elim ℕ encode (f b)⟩ : (a : α) × (β a → ℕ))
+      { exact this }
+      rw[Encodable.encode_sigma_val, Encodable.encode_sigma_val, encode_fintypeArrow, encode_finArrow, encode_list]
+      simp[Function.comp]; rw[←encode_finArrow, encode_fintypeArrow (β a)]; simp
+      congr; funext i; simp; rw[ih]; rfl }
+
+lemma encodeDecode_eq_elimDecode (s e : ℕ) : encodeDecode (SubWType β s) e = elimDecode β (fun a l => encode (a, l)) s e := by
+  simp[elimDecode, encodeDecode_eq_encode_map_decode]
+  rcases (decode e) <;> simp[encode_eq_elim']; congr
+  funext ⟨a, f⟩; simp[encode_fintypeArrow, encode_finArrow]
+
+instance uniformlyPrimcodable : UniformlyPrimcodable (SubWType β) :=
+  UniformlyPrimcodable.ofEncodeDecode (by
+    have : Primrec₂ (elimDecode β (fun a l => encode (a, l))) :=
+      primrec_elimDecode β (Primrec.encode.comp $ Primrec₂.pair.comp fst snd)
+    exact this.of_eq (by simp[encodeDecode_eq_elimDecode]))
+
+lemma depth_eq_elimDecode (s e : ℕ) :
+    (decode e : Option (SubWType β s)).map (fun w => w.val.depth) = elimDecode β (fun a l => l.sup + 1) s e := by
+  have : ∀ w : SubWType β s, depth w.val = elim' ℕ (fun p => Finset.sup Finset.univ p.snd + 1) s w
+  { induction' s with s ih
+    · simp; intro ⟨w, h⟩; simpa using lt_of_lt_of_le (depth_pos w) h
+    · rintro ⟨⟨a, f⟩, hw⟩;
+      simp[depth, ih, elim', elim]
+      have : ∀ (b : β a), depth (f b) = elim ℕ (fun p => Finset.sup Finset.univ p.snd + 1) (f b) :=
+        fun b => ih ⟨f b, by simp[depth, Nat.succ_eq_add_one] at hw; exact hw b⟩
+      simp[this] }
+  simp[elimDecode, encodeDecode_eq_encode_map_decode]
+  rcases (decode e) <;> simp[this]; congr
+  funext ⟨a, f⟩; simp[List.sup_ofFn, fintypeArrowEquivFinArrow_eq]
+
+lemma depth_decode_primrec : Primrec₂ (fun s e => (decode e : Option (SubWType β s)).map (fun w => w.val.depth)) := by
+  have : Primrec₂ (elimDecode β (fun a l => l.sup + 1)) :=
+    primrec_elimDecode β (by simp[←Nat.succ_eq_add_one]; apply Primrec.succ.comp $ (list_sup nat_max).comp snd)
+  exact this.of_eq (by simp[depth_eq_elimDecode])
+
+def ofW : WType β → (s : ℕ) × SubWType β s := fun w => ⟨w.depth, ofWType w w.depth (by rfl)⟩
+
+def toW : (s : ℕ) × SubWType β s → WType β := fun ⟨_, w⟩ => w.val
+
+end SubWType
+
+private lemma encode_decode_eq (e : ℕ) :
+    Option.casesOn ((decode e : Option ((s : ℕ) × SubWType β s)).map SubWType.toW) 0 (fun w => encode (SubWType.ofW w) + 1) =
+    encode (((encodeDecode (SubWType β e.unpair.1) e.unpair.2).bind
+      $ fun c => ((decode c : Option (SubWType β e.unpair.1)).map (fun w => w.val.depth)).map
+        $ fun d => d.pair c)) := by
+  simp[Function.comp, encodeDecode_eq_encode_map_decode]
+  rcases (decode e.unpair.2) with (_ | w) <;> simp[SubWType.toW, SubWType.ofW]
+  { simp[SubWType.encode_eq_elim']; apply SubWType.elim_const; simp }
+
+private lemma primrec_encode_decode :
+    Primrec (fun e => 
+      encode (((encodeDecode (SubWType β e.unpair.1) e.unpair.2).bind
+        $ fun c => ((decode c : Option (SubWType β e.unpair.1)).map (fun w => w.val.depth)).map
+          $ fun d => d.pair c)) : ℕ → ℕ) :=
+  (Primrec.encode.comp $
+    option_bind (Primrec₂.encodeDecode_u.comp (fst.comp Primrec.unpair) (snd.comp Primrec.unpair))
+      (option_map (SubWType.depth_decode_primrec.comp (fst.comp $ Primrec.unpair.comp fst) snd)
+        (Primrec₂.natPair.comp₂ Primrec₂.right (snd.comp fst))))
+
+private def encodable : Encodable (WType β) where
+  encode := fun w => encode (SubWType.ofW w)
+  decode := fun e => (decode e).map SubWType.toW
+  encodek := by rintro ⟨a, f⟩; simp[SubWType.toW, SubWType.ofW]
+
+instance _root_.Primcodable.wtype : Primcodable (WType β) :=
+  { encodable with
+    prim := Primrec.nat_iff.mp <| primrec_encode_decode.of_eq (fun e => (encode_decode_eq e).symm) }
+
+lemma encode_eq (w : WType β) : encode w = encode (SubWType.ofW w) := rfl
+
+lemma decode_eq (e : ℕ) : decode e = (decode e : Option ((s : ℕ) × SubWType β s)).map SubWType.toW := rfl
+
+def elimL (f : α → List γ → γ) : WType β → γ :=
+ fun w => elim γ (fun ⟨a, v⟩ => f a (List.ofFn $ fintypeArrowEquivFinArrow v)) w
+
+lemma elimL_mk (f : α → List γ → γ) (a : α) (v : β a → WType β) :
+    elimL f ⟨a, v⟩ = f a (List.ofFn $ fintypeArrowEquivFinArrow $ fun b => elimL f (v b)) := by simp[elimL, elim]
+
+lemma elim_eq_elimL [Inhabited γ] (f : (a : α) × (β a → γ) → γ) :
+    elim γ f w = elimL (fun a l => f ⟨a, fintypeArrowEquivFinArrow.symm (fun i => l.getI i)⟩) w := by
+  simp[elimL]; congr; funext ⟨a, j⟩; simp; congr; funext b; simp
+
+lemma decode_elimL_eq (f : α → List γ → γ) :
+    (decode e : Option (WType β)).map (elimL f) = (SubWType.elimDecode β f e.unpair.1 e.unpair.2) := by
+  simp[elimL, decode_eq, Function.comp, SubWType.elimDecode, SubWType.elim']
+  rcases (decode e.unpair.2) with (_ | ⟨_, _⟩) <;> simp[SubWType.toW]
+
+def mkL (a : α) (l : List (WType β)) : Option (WType β) :=
+  if h : l.length = Fintype.card (β a) then
+    some (WType.mk a $ fintypeArrowEquivFinArrow.symm $ fun (i : Fin (Fintype.card (β a))) => l.get (i.cast h.symm)) else none
+
+def mkFintype (a : α) (v : β a → WType β) : WType β := WType.mk a v
+
+def mk₀ (a : α) : Option (WType β) := mkL a []
+
+def mk₁ (a : α) (w : WType β) : Option (WType β) := mkL a [w]
+
+def mkFin {k} (a : α) (v : Fin k → WType β) : Option (WType β) := mkL a (List.ofFn v)
+
+lemma encode_mk_eq (a : α) (f : β a → WType β) :
+    encode (mk a f) = (Finset.sup Finset.univ (fun n => (f n).depth) + 1).pair ((encode a).pair (encode $ fun b => (encode $ f b).unpair.2)) := by
+  simp[encode_eq, SubWType.ofW, depth, SubWType.encode_mk]
+  funext b; simp[SubWType.encode_eq_elim']; apply SubWType.elim_const; simp
+
+lemma mk₀_eq (a : α) [h : IsEmpty (β a)] : mk₀ a = some (⟨a, h.elim'⟩ : WType β) := by
+  simp[mk₀, mkL, Fintype.card_eq_zero_iff.mpr h]
+
+end WType
+
+namespace Primrec
+
+open Encodable WType
+variable {σ : Type*} {α : Type*} {β : α → Type*} {γ : Type*}
+  [Primcodable σ] [Primcodable α] [(a : α) → Fintype (β a)]
+  [(a : α) → DecidableEq (β a)] [(a : α) → Primcodable (β a)] [PrimrecCard β] [Primcodable γ]
+
+lemma finArrow_list_ofFn {α} [Primcodable α] : Primrec (fun v => List.ofFn v : (Fin k → α) → List α) :=
+  have : Primrec (fun e => Encodable.encode $ Encodable.decode (α := Fin k → α) e) := Primrec.encode.comp Primrec.decode
+  (decode_iff.mp $ encode_iff.mp $ this.of_eq $ fun e => by rcases (Encodable.decode e) <;> simp[Encodable.encode_finArrow])
+
+lemma sigma_finArrow_list_ofFn {α} [Primcodable α] : Primrec (fun v => List.ofFn v.2 : (Σ k, Fin k → α) → List α) :=
+  have : Primrec (fun p => (encode p).unpair.2 : (Σ k, Fin k → α) → ℕ) := (snd.comp $ unpair.comp Primrec.encode)
+  encode_iff.mp (this.of_eq $ fun ⟨k, v⟩ => by simp[encode_finArrow])
+
+lemma sigma_fst [UniformlyPrimcodable β] : Primrec (Sigma.fst : ((a : α) × β a) → α) :=
+  have : Primrec (fun e => (decode (α := α) e.unpair.1).bind $ fun a => (encodeDecode (β a) e.unpair.2).map (fun _ => a) : ℕ → Option α) :=
+    option_bind (Primrec.decode.comp $ fst.comp unpair)
+      (option_map (Primrec₂.encodeDecode_u.comp snd (snd.comp $ unpair.comp fst)) (snd.comp fst).to₂)
+  decode_iff.mp (this.of_eq $
+    by intro n; simp; rcases (decode n.unpair.1) with (_ | a) <;> simp
+       { simp[encodeDecode_eq_encode_map_decode, Function.comp] })
+
+lemma sigma_prod_left {α} {β γ : α → Type*} [Primcodable α]
+  [(a : α) → Primcodable (β a)] [(a : α) → Primcodable (γ a)] [UniformlyPrimcodable β] [UniformlyPrimcodable γ] :
+    Primrec (fun p => ⟨p.1, p.2.1⟩ : (Σ a, β a × γ a) → (Σ a, β a)) :=
+  have : Primrec (fun p => Nat.pair (encode p).unpair.1 (encode p).unpair.2.unpair.1 : (Σ a, β a × γ a) → ℕ) :=
+    Primrec₂.natPair.comp (fst.comp $ unpair.comp Primrec.encode) (fst.comp $ unpair.comp $ snd.comp $ unpair.comp Primrec.encode)
+  encode_iff.mp (this.of_eq $ fun ⟨k, b, v⟩ => by simp[encode_finArrow])
+
+lemma sigma_prod_right {α} {β γ : α → Type*} [Primcodable α]
+  [(a : α) → Primcodable (β a)] [(a : α) → Primcodable (γ a)] [UniformlyPrimcodable β] [UniformlyPrimcodable γ] :
+    Primrec (fun p => ⟨p.1, p.2.2⟩ : (Σ a, β a × γ a) → (Σ a, γ a)) :=
+  have : Primrec (fun p => Nat.pair (encode p).unpair.1 (encode p).unpair.2.unpair.2 : (Σ a, β a × γ a) → ℕ) :=
+    Primrec₂.natPair.comp (fst.comp $ unpair.comp Primrec.encode) (snd.comp $ unpair.comp $ snd.comp $ unpair.comp Primrec.encode)
+  encode_iff.mp (this.of_eq $ fun ⟨k, b, v⟩ => by simp[encode_finArrow])
+
+lemma sigma_pair [UniformlyPrimcodable β] (a : α) : Primrec (Sigma.mk a : β a → (a : α) × β a) :=
+  encode_iff.mp (by simp; exact Primrec₂.natPair.comp (const _) Primrec.encode)
+
+lemma finArrow_map {f} (hf : Primrec f) (k) : Primrec (fun v i => f (v i) : (Fin k → α) → (Fin k → σ)) := by
+  have : Primrec (fun e => encode $ ((encodeDecode (Fin k → α) e).bind
+    $ fun c => (decode c : Option (List α)).map (fun l => l.map f)) : ℕ → ℕ) :=
+    (Primrec.encode.comp $ option_bind Primrec.encodeDecode
+      (option_map (Primrec.decode.comp snd) (by apply list_map snd (hf.comp₂ Primrec₂.right))))
+  exact decode_iff.mp (encode_iff.mp $ this.of_eq $ fun e => by
+    simp[encodeDecode_eq_encode_map_decode, decode_finArrow]
+    rcases has : (decode e) with (_ | as) <;> simp[Function.comp]
+    { rfl }
+    { rcases hv : (as.toVector k) with (_ | v) <;> simp
+      { rfl }
+      { rw[Encodable.encode_some]; simp[encode_finArrow, Function.comp] } })
+
+lemma w_depth : Primrec (fun w => w.depth : WType β → ℕ) := by
+  have : Primrec (fun n => (encodeDecode (WType β) n).map $ fun e => e.unpair.1) :=
+    option_map Primrec.encodeDecode (fst.comp₂ $ Primrec.unpair.comp₂ Primrec₂.right)
+  exact decode_iff.mp (this.of_eq $ fun n => by
+    simp[encodeDecode_eq_encode_map_decode]
+    rcases decode n <;> simp[WType.encode_eq, WType.SubWType.ofW])
+
+lemma w_elimL {f : α → List γ → γ} (hf : Primrec₂ f) : Primrec (elimL f : WType β → γ) :=
+  decode_iff.mp (by simp[decode_elimL_eq]; apply SubWType.primrec_elimDecode β hf)
+
+lemma w_elimL_param {f : σ → α × List γ → γ} (hf : Primrec₂ f) : Primrec₂ (fun x w => elimL (fun p l => f x (p, l)) w : σ → WType β → γ) :=
+  Primrec₂.decode_iff₂.mp
+    (by simp[decode_elimL_eq]
+        exact (SubWType.primrec_elimDecode_param β hf).comp₂ Primrec₂.left
+          (Primrec.pair (fst.comp $ Primrec.unpair.comp snd) (snd.comp $ Primrec.unpair.comp snd)).to₂)
+
+lemma w_elim [Inhabited γ] {f : (a : α) × (β a → γ) → γ}
+  (hf : Primrec₂ (fun a l => f ⟨a, fintypeArrowEquivFinArrow.symm (fun i => l.getI i)⟩ : α → List γ → γ)) :
+    Primrec (WType.elim γ f) := (w_elimL (β := β) hf).of_eq (fun w => by simp[elim_eq_elimL])
+
+lemma w_elim_param [Inhabited γ] {f : σ → (a : α) × (β a → γ) → γ}
+  (hf : Primrec₂ (fun x p => f x ⟨p.1, fintypeArrowEquivFinArrow.symm (fun i => p.2.getI i)⟩ : σ → α × List γ → γ)) :
+    Primrec₂ (fun x => WType.elim γ (f x)) := (w_elimL_param (β := β) hf).of_eq (fun x w => by simp[elim_eq_elimL])
+
+lemma w_mkL : Primrec₂ (WType.mkL : α → List (WType β) → Option (WType β)) :=
+  have : Primrec₂ (fun a l => if l.length = Fintype.card (β a)
+      then ((l.map depth).sup + 1).pair ((encode a).pair (encode $ l.map (fun w => (encode w).unpair.2))) + 1
+      else 0 : α → List (WType β) → ℕ) :=
+    Primrec.ite (Primrec.eq.comp (list_length.comp snd) (PrimrecCard.card_prim.comp fst))
+      (succ.comp $ Primrec₂.natPair.comp
+        (succ.comp $ (list_sup nat_max).comp $ list_map snd (w_depth.comp snd))
+        (Primrec₂.natPair.comp (Primrec.encode.comp fst)
+          (Primrec.encode.comp $ list_map snd (snd.comp $ unpair.comp $ Primrec.encode.comp snd))))
+      (const 0)
+  Primrec₂.encode_iff.mp (this.of_eq $ fun a l => by
+  { by_cases h : l.length = Fintype.card (β a) <;> simp[WType.mkL, *]
+    { simp[encode_mk_eq]; constructor
+      { exact Eq.trans (by rw[Finset.sup_univ_cast (fun i => depth (l.get i))]; exact Eq.symm <| Finset.sup_univ_list_eq_sup_map _ _)
+          (Eq.symm <| Finset.sup_univ_equiv (fun i => depth (l.get (i.cast h.symm)) : Fin (Fintype.card (β a)) → ℕ) fintypeEquivFin) }
+      { simp[encode_fintypeArrow, encode_finArrow]
+        ext i c; simp
+        rcases hw : (l.get? i) with (_ | w) <;> simp[List.ofFnNthVal]
+        · have : ¬i < Fintype.card (β a) := by simpa[h] using List.get?_eq_none.mp hw
+          simp[this]
+        · have : ∃ hi, l.get ⟨i, hi⟩ = w := List.get?_eq_some.mp hw
+          rcases this with ⟨hi, rfl⟩
+          have : i < Fintype.card (β a) := by simpa[h] using hi
+          simp[this] } } })
+
+lemma w_mk₀ (f : σ → α) (h : (x : σ) → IsEmpty (β (f x))) (hf : Primrec f) {v : {x : σ} → β (f x) → WType β}:
+    Primrec (fun x => WType.mk (f x) v : σ → WType β) := by
+  have : Primrec (fun x => Nat.pair 1 (Nat.pair (encode $ f x) 0) : σ → ℕ) :=
+    Primrec₂.natPair.comp (const 1) (Primrec₂.natPair.comp (Primrec.encode.comp hf) (const 0))
+  exact Primrec.encode_iff.mp (this.of_eq $ fun x => by simp[encode_mk_eq, encode_fintypeArrow_isEmpty])
+
+lemma w_mk₁ (f : σ → α) (h : ∀ x, Fintype.card (β (f x)) = 1) (hf : Primrec f) :
+    Primrec₂ (fun x w => WType.mk (f x) (fun _ => w) : σ → WType β → WType β) := by
+  have : Primrec₂ (fun x w => Nat.pair (w.depth + 1) (Nat.pair (encode $ f x) (encode [(encode w).unpair.2])) : σ → WType β → ℕ) :=
+    Primrec₂.natPair.comp
+      (succ.comp $ w_depth.comp snd)
+      (Primrec₂.natPair.comp (Primrec.encode.comp $ hf.comp fst)
+        (Primrec.encode.comp $ list_cons.comp (snd.comp $ unpair.comp $ Primrec.encode.comp snd) (const [])))
+  exact Primrec₂.encode_iff.mp (this.of_eq $ fun x w => by
+    simp[encode_mk_eq, encode_fintypeArrow_card_one (h x) ℕ _ (fintypeEquivFin.symm ((0 : Fin 1).cast (h x).symm))]
+    have : Finset.univ = {fintypeEquivFin.symm ((0 : Fin 1).cast (h x).symm)}
+    { have : Subsingleton (β (f x)) := Fintype.card_le_one_iff_subsingleton.mp (by simp[h x])
+      ext; simp }
+    rw[this, Finset.sup_singleton])
+
+lemma w_mk₂ (f : σ → α) (h : ∀ x, Fintype.card (β (f x)) = 2) (hf : Primrec f) :
+    Primrec₂ (fun x w => WType.mk (f x) ((fintypeArrowEquivFinArrow' (h x)).symm ![w.1, w.2]) : σ → WType β × WType β → WType β) := by
+  have : Primrec₂ (fun x w => Nat.pred $ encode (WType.mkL (f x) [w.1, w.2]) : σ → WType β × WType β → ℕ) :=
+    (pred.comp $ Primrec.encode.comp $ w_mkL.comp (hf.comp fst) (list_cons.comp (fst.comp snd) (list_cons.comp (snd.comp snd) (const []))))
+  exact Primrec₂.encode_iff.mp (this.of_eq $ fun x ⟨w₁, w₂⟩ => by
+    simp[mkL, h]
+    have := (fintypeArrowEquivFinArrow' (α := WType β) (h x)).injective
+    apply this
+    funext i; simp
+    cases i using Fin.cases <;> simp)
+
+lemma w_mkFin (f : σ → α) {k} (h : ∀ x, Fintype.card (β (f x)) = k) (hf : Primrec f) :
+    Primrec₂ (fun x w => WType.mk (f x) ((fintypeArrowEquivFinArrow' (h x)).symm w) : σ → (Fin k → WType β) → WType β) := by
+  have : Primrec₂ (fun x w => Nat.pred $ encode (WType.mkL (f x) (List.ofFn w)) : σ → (Fin k → WType β) → ℕ) :=
+    (pred.comp $ Primrec.encode.comp $ w_mkL.comp (hf.comp fst) (finArrow_list_ofFn.comp snd))
+  exact Primrec₂.encode_iff.mp (this.of_eq $ fun x w => by
+    simp[mkL, h]
+    have := (fintypeArrowEquivFinArrow' (α := WType β) (h x)).injective
+    apply this
+    funext i; simp; congr)
+
+end Primrec
